\begin{problem}{1}
\end{problem}
\begin{solution}
We directly apply the definition of conditional probability:
\begin{align*}
    \Pr[\omega_1 = 1 | \omega_1 + \ldots + \omega_n = m] &= \frac{\Pr[\omega_1 = 1 \cap \omega_1 + \ldots + \omega_n = m]}{\Pr[\omega_1 + \ldots + \omega_n = m]}, \\
    &= \frac{\binom{n-1}{m-1}p^m(1-p)^{n-m}}{\binom{n}{m}p^m(1-p)^{n-m}}, \\
    &= \binom{n-1}{m-1} \big/ \binom{n}{m}, \\
    &= \frac{m}{n}.
\end{align*}
\end{solution}
\begin{problem}{2}
\end{problem}
\begin{solution}
    We are looking for a distribution that is \textit{memoryless}, both the exponential distribution and the Poisson distribution satisfy this property. Let $\xi$ be a exponentially-distributed random variable, parameterized by $\lambda$. Then, 
    $\Pr[\xi > x] = e^{-\lambda x}$ and 
    \begin{align*}
        \Pr[\xi > x+y | \xi > x] &= \frac{\Pr[\xi > x+y]}{\Pr[\xi > x]}, \\
        &= \frac{e^{-\lambda(x+y)}}{e^{-\lambda x}}, \\
        &= e^{-\lambda y}.
    \end{align*}
\end{solution}
\begin{problem}{3}
\end{problem}
\begin{solution}
    Let $H^1, H^2$ denote the event that heads appears on the first and second toss, respectively. Then,
    \begin{align*}
        \Pr[H^2|H^1] &= \frac{\Pr[H^1 \cap H^2]}{\Pr[H^1]}, \\
        &= \frac{1/2(1/2^2) + 1/2(0.6^2)}{1/2(1/2) + 1/2(0.6)}, \\
        &= 0.55.
    \end{align*}
\end{solution}
\begin{problem}{4}
\end{problem}
\begin{solution}
    Suppose that $\xi,\eta$ are two random variables such that both of their images is $\{a,b\}$. We show then that if $\Exp{\xi\eta} = \Exp{\xi}\Exp{\eta}$, then $\eta$ and $\xi$ are independent. Let $p,q$ be the probability that $\xi = a,\eta=a$, respectively. Then, 
    \begin{align*}
        \Exp{\xi}\Exp{\eta} &= (pa + (1-p)b)(qa + (1-q)b), \\
        &= a^2pq + ab(p)(1-q) + ba(q)(1-p) + b^2(1-p)(1-q), \\
        \Exp{\xi\eta} &= a\Pr[\eta=a,\xi=a] + ab\Pr[\eta=a,\xi=b] + ba\Pr[\eta=b,\xi=a] + b^2\Pr[\xi=b,\eta=b],
    \end{align*}
    This implies that 
    \begin{align*}
        \Pr[\xi=a,\eta=a] &= pq = \Pr[\xi=a]\Pr[\eta=a], \\
        \Pr[\xi=b,\eta=b] &= (1-q)(1-p) = \Pr[\xi=b]\Pr[\eta=b].
    \end{align*}
    By Lemma 4.3, then events $\xi = a, \eta = b$ and $\eta=a,\xi=b$ are also independent. 
\end{solution}
\begin{problem}{5}
\end{problem}
\begin{solution}
    
\end{solution}
\begin{problem}{6}
\end{problem}
\begin{solution}
    
\end{solution}
\begin{problem}{7}

\end{problem}
\begin{solution}
    
\end{solution}