\begin{lemma}\label{lem:matrix-product}
    Let $P \in \R^{r\times r}$ and denote the $i,j$ entry of $P$ as $P_{i,j}$. Then, 
    \[
        P^S_{i,j} = \sum_{i_1=1}^r \cdots \sum_{i_S=1}^r P_{i,i_1} \cdots P_{i_{S-1},j},
    \]
    for all $S \geq 2$. 
\end{lemma}
\begin{proof}
    We proceed by way of induction on $S$. The equality trivially holds when $S=2$ since by the definition of matrix multiplication:
    \[
        P^2_{i,j} = \sum_{k=1}^r P_{i,k}P_{k,j}.    
    \] 
    Suppose the statement true for all $n>2$. Then, 
    \begin{align*}
        P^{n+1}_{i,j} &= (P^n\cdot P)_{i,j}, \\
        &= \sum_{k=1}^r P^n_{i,k}P_{k,j}, \\
        &= \sum_{k=1}^r \sum_{i_1=1}^r\cdots \sum_{i_n=1}^r P_{i,i_1}\cdots P_{i_n,k} P_{k,j}, \\
        &= \sum_{i_1=1}^r\cdots \sum_{i_{n+1}=1}^r P_{i,i_1} \cdots P_{i_n,i_{n+1}}P_{i_{n+1},j}.
    \end{align*}
    The last equality comes from relabeling.
\end{proof}
\begin{corollary}\label{cor:initial-dist}
    If $\mu \in \R^{1\times r}$, then 
    \[
        (\mu P^S)_k = \sum_{i=1}^r \sum_{i_1=1}^r \cdots \sum_{i_S=1}^r \mu_i  P_{i,i_1} \cdots P_{i_{S-1},k}.
    \]
\end{corollary}
\begin{proof}
    By definition of vector-matrix multiplication, 
    \begin{align*}
        (\mu P^S)_k &= \sum_{i=1}^r \mu_i\cdot P_{i,k}^S, \\ 
        &= \sum_{i=1}^r \mu_i \cdot \sum_{i_1=1}^r \cdots \sum_{i_S=1}^r P_{i,i_1} \cdots P_{i_{S-1},k},  \\
        &=\sum_{i=1}^r \sum_{i_1=1}^r \cdots \sum_{i_S=1}^r \mu_i  P_{i,i_1} \cdots P_{i_{S-1},k}.
    \end{align*}
    The second equality follows from Lemma~\ref{lem:matrix-product}.
\end{proof}